Add Blake2 pad and finish to agile implementations

code/hash/Hacl.Hash.Definitions.fst
@@ -6,6 +6,7 @@ module ST = FStar.HyperStack.ST
 module M = LowStar.Modifies
 module B = LowStar.Buffer
 module Spec = Spec.Hash.PadFinish
+module Blake2 = Hacl.Impl.Blake2.Core
 
 open Lib.IntTypes
 open Spec.Hash.Definitions
@@ -14,21 +15,59 @@ open FStar.Mul
 (** The low-level types that our clients need to be aware of, in order to
     successfully call this module. *)
 
+inline_for_extraction noextract
+let impl_word (a:hash_alg) = match a with
+  | MD5 | SHA1 | SHA2_224 | SHA2_256 | SHA2_384 | SHA2_512 -> word a
+  | Blake2S | Blake2B -> Blake2.element_t (to_blake_alg a) Blake2.M32
+
+inline_for_extraction noextract
+let impl_state_length (a:hash_alg) = match a with
+  | MD5 | SHA1 | SHA2_224 | SHA2_256 | SHA2_384 | SHA2_512 -> state_word_length a
+  | Blake2S | Blake2B -> UInt32.v (4ul *. Blake2.row_len (to_blake_alg a) Blake2.M32)
+
+inline_for_extraction noextract
+type state_l (a:hash_alg) = b:B.buffer (impl_word a) { B.length b = impl_state_length a }
+
 inline_for_extraction
 type state (a: hash_alg) =
-  b:B.buffer (word a) { B.length b = state_word_length a }
+  state_l a & B.pointer (extra_state a)
+
+inline_for_extraction noextract
+let invariant (#a: hash_alg) (h:HS.mem) (s:state a) =
+  let s, p = s in
+  B.live h s /\ B.live h p /\ B.disjoint s p
+
+inline_for_extraction noextract
+let footprint (#a:hash_alg) (s:state a) =
+   B.loc_buffer (fst s) `B.loc_union` B.loc_buffer (snd s)
+
+inline_for_extraction noextract
+let as_seq_l (#a:hash_alg) (h:HS.mem) (s:state_l a) : GTot (words_state' a) =
+  match a with
+  | MD5 | SHA1 | SHA2_224 | SHA2_256 | SHA2_384 | SHA2_512 -> B.as_seq h s
+  | Blake2S -> Blake2.state_v #Spec.Blake2.Blake2S #Blake2.M32 h s
+  | Blake2B -> Blake2.state_v #Spec.Blake2.Blake2B #Blake2.M32 h s
+
+
+inline_for_extraction noextract
+let as_seq (#a:hash_alg) (h:HS.mem) (s:state a) : GTot (words_state a) =
+  as_seq_l h (fst s), B.deref h (snd s)
 
 inline_for_extraction
 let word_len (a: hash_alg): n:size_t { v n = word_length a } =
   match a with
   | MD5 | SHA1 | SHA2_224 | SHA2_256 -> 4ul
   | SHA2_384 | SHA2_512 -> 8ul
+  | Blake2S -> 4ul
+  | Blake2B -> 8ul
 
 inline_for_extraction
 let block_len (a: hash_alg): n:size_t { v n = block_length a } =
   match a with
   | MD5 | SHA1 | SHA2_224 | SHA2_256 -> 64ul
   | SHA2_384 | SHA2_512 -> 128ul
+  | Blake2S -> 64ul
+  | Blake2B -> 128ul
 
 inline_for_extraction
 let hash_word_len (a: hash_alg): n:size_t { v n = hash_word_length a } =
@@ -39,6 +78,7 @@ let hash_word_len (a: hash_alg): n:size_t { v n = hash_word_length a } =
   | SHA2_256 -> 8ul
   | SHA2_384 -> 6ul
   | SHA2_512 -> 8ul
+  | Blake2S | Blake2B -> 8ul
 
 inline_for_extraction
 let hash_len (a: hash_alg): n:size_t { v n = hash_length a } =
@@ -49,6 +89,8 @@ let hash_len (a: hash_alg): n:size_t { v n = hash_length a } =
   | SHA2_256 -> 32ul
   | SHA2_384 -> 48ul
   | SHA2_512 -> 64ul
+  | Blake2S -> 32ul
+  | Blake2B -> 64ul
 
 inline_for_extraction
 let blocks_t (a: hash_alg) =
@@ -65,18 +107,20 @@ let alloca_st (a: hash_alg) = unit -> ST.StackInline (state a)
     HS.is_stack_region (HS.get_tip h)))
   (ensures (fun h0 s h1 ->
     M.(modifies M.loc_none h0 h1) /\
-    B.live h1 s /\
-    B.frameOf s == HS.get_tip h0 /\
-    Seq.equal (B.as_seq h1 s) (fst (Spec.Agile.Hash.init a)) /\
-    LowStar.Monotonic.Buffer.alloc_post_mem_common s h0 h1 (fst (Spec.Agile.Hash.init a))))
+    B.frameOf (fst s) == HS.get_tip h0 /\
+    B.frameOf (snd s) == HS.get_tip h0 /\
+    invariant h1 s /\
+    as_seq h1 s == Spec.Agile.Hash.init a /\
+    Map.domain (HS.get_hmap h1) `Set.equal` Map.domain (HS.get_hmap h0) /\
+    (HS.get_tip h1) == (HS.get_tip h0) /\
+    B.unused_in (fst s) h0 /\ B.unused_in (snd s) h0))
 
 inline_for_extraction
 let init_st (a: hash_alg) = s:state a -> ST.Stack unit
-  (requires (fun h ->
-    B.live h s))
+  (requires (fun h -> invariant h s))
   (ensures (fun h0 _ h1 ->
-    M.(modifies (loc_buffer s) h0 h1) /\
-    Seq.equal (B.as_seq h1 s) (fst (Spec.Agile.Hash.init a))))
+    M.(modifies (footprint s) h0 h1) /\
+    as_seq h1 s == Spec.Agile.Hash.init a))
 
 inline_for_extraction
 let update_st (a: hash_alg) =
@@ -84,10 +128,10 @@ let update_st (a: hash_alg) =
   block:B.buffer uint8 { B.length block = block_length a } ->
   ST.Stack unit
     (requires (fun h ->
-      B.live h s /\ B.live h block /\ B.disjoint s block))
+      invariant h s /\ B.live h block /\ B.loc_disjoint (footprint s) (B.loc_buffer block)))
     (ensures (fun h0 _ h1 ->
-      M.(modifies (loc_buffer s) h0 h1) /\
-      Seq.equal (B.as_seq h1 s) (fst (Spec.Agile.Hash.update a (B.as_seq h0 s, ()) (B.as_seq h0 block)))))
+      M.(modifies (footprint s) h0 h1) /\
+      as_seq h1 s == (Spec.Agile.Hash.update a (as_seq h0 s) (B.as_seq h0 block))))
 
 inline_for_extraction
 let pad_st (a: hash_alg) = len:len_t a -> dst:B.buffer uint8 ->
@@ -109,11 +153,10 @@ let update_multi_st (a: hash_alg) =
   n:size_t { B.length blocks = block_length a * v n } ->
   ST.Stack unit
     (requires (fun h ->
-      B.live h s /\ B.live h blocks /\ B.disjoint s blocks))
+      invariant h s /\ B.live h blocks /\ B.loc_disjoint (footprint s) (B.loc_buffer blocks)))
     (ensures (fun h0 _ h1 ->
-      B.(modifies (loc_buffer s) h0 h1) /\
-      Seq.equal (B.as_seq h1 s)
-        (fst (Spec.Agile.Hash.update_multi a (B.as_seq h0 s, ()) (B.as_seq h0 blocks)))))
+      B.(modifies (footprint s) h0 h1) /\
+      as_seq h1 s == Spec.Agile.Hash.update_multi a (as_seq h0 s) (B.as_seq h0 blocks)))
 
 inline_for_extraction
 let update_last_st (a: hash_alg) =
@@ -123,21 +166,18 @@ let update_last_st (a: hash_alg) =
   input_len:size_t { B.length input = v input_len } ->
   ST.Stack unit
     (requires (fun h ->
-      B.live h s /\ B.live h input /\ B.disjoint s input))
+      invariant h s /\ B.live h input /\ B.loc_disjoint (footprint s) (B.loc_buffer input)))
     (ensures (fun h0 _ h1 ->
-      B.(modifies (loc_buffer s) h0 h1) /\
-      Seq.equal (B.as_seq h1 s)
-        (fst (Spec.Hash.Incremental.update_last a (B.as_seq h0 s, ()) (len_v a prev_len) (B.as_seq h0 input)))))
+      B.(modifies (footprint s) h0 h1) /\
+      as_seq h1 s == Spec.Hash.Incremental.update_last a (as_seq h0 s) (len_v a prev_len) (B.as_seq h0 input)))
 
 inline_for_extraction
 let finish_st (a: hash_alg) = s:state a -> dst:hash_t a -> ST.Stack unit
   (requires (fun h ->
-    B.disjoint s dst /\
-    B.live h s /\
-    B.live h dst))
+    invariant h s /\ B.live h dst /\ B.loc_disjoint (footprint s) (B.loc_buffer dst)))
   (ensures (fun h0 _ h1 ->
     M.(modifies (loc_buffer dst) h0 h1) /\
-    Seq.equal (B.as_seq h1 dst) (Spec.Hash.PadFinish.finish a (B.as_seq h0 s, ()))))
+    Seq.equal (B.as_seq h1 dst) (Spec.Hash.PadFinish.finish a (as_seq h0 s))))
 
 inline_for_extraction
 let hash_st (a: hash_alg) =
